refactor(field_theory/finite): generalize proofs (#429)

data/equiv/algebra.lean
@@ -3,7 +3,7 @@ Copyright (c) 2018 Johannes Hölzl. All rights reserved.
 Released under Apache 2.0 license as described in the file LICENSE.
 Authors: Johannes Hölzl
 -/
-import data.equiv.basic algebra.group
+import data.equiv.basic algebra.group algebra.field
 
 namespace equiv
 variables {α : Type*} [group α]
@@ -37,5 +37,11 @@ protected def inv (α) [group α] : α ≃ α :=
 attribute [to_additive equiv.neg._proof_1] equiv.inv._proof_1
 attribute [to_additive equiv.neg._proof_2] equiv.inv._proof_2
 attribute [to_additive equiv.neg] equiv.inv
+
+def units_equiv_ne_zero (α : Type*) [field α] : units α ≃ {a : α | a ≠ 0} :=
+⟨λ a, ⟨a.1, units.ne_zero _⟩, λ a, units.mk0 _ a.2, λ ⟨_, _, _, _⟩, units.ext rfl, λ ⟨_, _⟩, rfl⟩
+
+@[simp] lemma coe_units_equiv_ne_zero [field α] (a : units α) :
+  ((units_equiv_ne_zero α a) : α) = a := rfl
 
 end equiv
